

信号理論基礎 課題レポート 1

細川 夏風

2025 年 6 月 13 日

授業より, $a_m = \frac{1}{\int_0^4 (f_m)^2 dt} \int_0^4 f f_m dt$, $f_1 = \begin{bmatrix} 1 \\ 1 \\ 1 \\ 1 \end{bmatrix}$, $f_2 = \begin{bmatrix} 1 \\ 1 \\ -1 \\ -1 \end{bmatrix}$, $f_3 = \begin{bmatrix} 1 \\ -1 \\ -1 \\ 1 \end{bmatrix}$, $f_4 = \begin{bmatrix} 1 \\ -1 \\ 1 \\ -1 \end{bmatrix}$, を用いる.

(1). $f = \begin{bmatrix} 5 \\ 1 \\ -5 \\ 3 \end{bmatrix}$ のときの $a_1 \sim a_4$ を求めよ.

$$\begin{aligned} a_1 &= \frac{1}{4} \int_0^4 f f_1 dt \\ &= \frac{1}{4} \langle f, f_1 \rangle \\ &= \frac{1}{4} \{5 \cdot 1 + 1 \cdot 1 + (-5) \cdot 1 + 3 \cdot 1\} \\ &= \frac{1}{4} \cdot 4 \\ &= 1 \\ \text{よって } a_1 &= 1. \end{aligned}$$

$$\begin{aligned} a_2 &= \frac{1}{4} \int_0^4 f f_2 dt \\ &= \frac{1}{4} \langle f, f_2 \rangle \\ &= \frac{1}{4} \{5 \cdot 1 + 1 \cdot 1 + (-5) \cdot (-1) + 3 \cdot (-1)\} \\ &= \frac{1}{4} \cdot 8 \\ &= 2 \\ \text{よって } a_2 &= 2. \end{aligned}$$

$$\begin{aligned} a_3 &= \frac{1}{4} \int_0^4 f f_3 dt \\ &= \frac{1}{4} \langle f, f_3 \rangle \\ &= \frac{1}{4} \{5 \cdot 1 + 1 \cdot (-1) + (-5) \cdot (-1) + 3 \cdot 1\} \\ &= \frac{1}{4} \cdot 12 \\ &= 3 \\ \text{よって } a_3 &= 3. \end{aligned}$$

$$\begin{aligned} a_4 &= \frac{1}{4} \int_0^4 f f_4 dt \\ &= \frac{1}{4} \langle f, f_4 \rangle \\ &= \frac{1}{4} \{5 \cdot 1 + 1 \cdot (-1) + (-5) \cdot 1 + 3 \cdot (-1)\} \\ &= \frac{1}{4} \cdot (-4) \\ &= -1 \\ \text{よって } a_4 &= -1. \end{aligned}$$

(2). $f = \begin{bmatrix} 4 \\ 0 \\ 0 \\ 0 \end{bmatrix}$ のときの $a_1 \sim a_4$ を求めよ.

$$\begin{aligned}
 a_1 &= \frac{1}{4} \int_0^4 f f_1 dt \\
 &= \frac{1}{4} \langle f, f_1 \rangle \\
 &= \frac{1}{4} \{4 \cdot 1 + 0 \cdot 1 + 0 \cdot 1 + 0 \cdot 1\} \\
 &= \frac{1}{4} \cdot 4 \\
 &= 1 \\
 &\text{よって } a_1 = 1.
 \end{aligned}$$

$$\begin{aligned}
 a_2 &= \frac{1}{4} \int_0^4 f f_2 dt \\
 &= \frac{1}{4} \langle f, f_2 \rangle \\
 &= \frac{1}{4} \{4 \cdot 1 + 0 \cdot 1 + 0 \cdot (-1) + 0 \cdot (-1)\} \\
 &= \frac{1}{4} \cdot 4 \\
 &= 1 \\
 &\text{よって } a_2 = 1.
 \end{aligned}$$

$$\begin{aligned}
 a_3 &= \frac{1}{4} \int_0^4 f f_3 dt \\
 &= \frac{1}{4} \langle f, f_3 \rangle \\
 &= \frac{1}{4} \{4 \cdot 1 + 0 \cdot (-1) + 0 \cdot (-1) + 0 \cdot 1\} \\
 &= \frac{1}{4} \cdot 4 \\
 &= 1 \\
 &\text{よって } a_3 = 1.
 \end{aligned}$$

$$\begin{aligned}
 a_4 &= \frac{1}{4} \int_0^4 f f_4 dt \\
 &= \frac{1}{4} \langle f, f_4 \rangle \\
 &= \frac{1}{4} \{4 \cdot 1 + 0 \cdot (-1) + 0 \cdot 1 + 0 \cdot (-1)\} \\
 &= \frac{1}{4} \cdot 4 \\
 &= 1 \\
 &\text{よって } a_4 = 1.
 \end{aligned}$$

参考文献

[1] 無し